ulib/FStar.Reflection.Syntax.fst
@@ -1,0 +1,218 @@
+module FStar.Reflection.Syntax
+open FStar.Order
+
+assume val term : Type0
+
+assume val fv : Type0
+assume val binder : Type0 // really a bv, qualifiers are ignored, unsure they're really needed
+assume val env : Type0// would maybe make more sense in tactics, as they're special cased
+
+type name    = list string
+type typ     = term
+type binders = list binder
+
+noeq
+type const =
+  | C_Unit : const
+  | C_Int : int -> const // Not exposing the details, I presume
+  | C_True : const
+  | C_False : const
+  (* TODO: complete *)
+
+noeq
+type term_view =
+  | Tv_Var    : binder -> term_view
+  | Tv_FVar   : fv -> term_view
+  | Tv_App    : term -> term -> term_view
+  | Tv_Abs    : binder -> term -> term_view
+  | Tv_Arrow  : binder -> term -> term_view
+  | Tv_Type   : unit -> term_view
+  | Tv_Refine : binder -> term -> term_view
+  | Tv_Const  : const -> term_view
+  | Tv_Unknown : term_view // Baked in "None"
+  (* TODO: complete *)
+
+assume private val __type_of_binder: binder -> term
+let type_of_binder (b:binder) : term = __type_of_binder b
+
+(* Comparison of a term_view to term. Allows to recurse while changing the view *)
+val smaller : term_view -> term -> Type0
+let smaller tv t =
+    match tv with
+    | Tv_App l r ->
+        l << t /\ r << t
+
+    | Tv_Abs b t'
+    | Tv_Arrow b t'
+    | Tv_Refine b t' ->
+        type_of_binder b << t /\ t' << t
+
+    | Tv_Type _
+    | Tv_Const _
+    | Tv_Unknown
+    | Tv_Var _
+    | Tv_FVar _ -> True
+
+(* The main characters *)
+assume val __inspect : t:term -> tv:term_view{smaller tv t}
+let inspect t : term_view = __inspect t
+
+assume val __pack : term_view -> term
+let pack tv : term = __pack tv
+
+(* They are inverses *)
+assume val pack_inspect_inv : (t:term) -> Lemma (pack (inspect t) == t)
+assume val inspect_pack_inv : (tv:term_view) -> Lemma (inspect (pack tv) == tv)
+
+assume val __inspect_fv : fv -> name
+let inspect_fv (fv:fv) = __inspect_fv fv
+
+assume val __pack_fv : name -> fv
+let pack_fv (ns:name) = __pack_fv ns
+
+assume val __compare_binder : binder -> binder -> order
+let compare_binder (b1:binder) (b2:binder) = __compare_binder b1 b2
+
+assume val __inspect_bv : binder -> string
+let inspect_bv (b:binder) = __inspect_bv b
+
+assume private val __binders_of_env : env -> binders
+let binders_of_env (e:env) : binders = __binders_of_env e
+
+assume private val __is_free : binder -> term -> bool
+let is_free (b:binder) (t:term) : bool = __is_free b t
+
+assume private val __term_eq : term -> term -> bool
+let term_eq t1 t2 : bool = __term_eq t1 t2
+
+assume val __term_to_string : term -> string
+let term_to_string t : string = __term_to_string t
+
+assume val __fresh_binder : typ -> binder
+let fresh_binder t : binder = __fresh_binder t
+
+val flatten_name : name -> Tot string
+let rec flatten_name ns =
+    match ns with
+    | [] -> ""
+    | [n] -> n
+    | n::ns -> n ^ "." ^ flatten_name ns
+
+
+// TODO: these are awful names
+let imp_qn       = ["Prims"; "l_imp"]
+let and_qn       = ["Prims"; "l_and"]
+let or_qn        = ["Prims"; "l_or"]
+let not_qn       = ["Prims"; "l_not"]
+let iff_qn       = ["Prims"; "l_iff"]
+let eq2_qn       = ["Prims"; "eq2"]
+let eq1_qn       = ["Prims"; "eq"]
+let true_qn      = ["Prims"; "l_True"]
+let false_qn     = ["Prims"; "l_False"]
+let b2t_qn       = ["Prims"; "b2t"]
+let forall_qn    = ["Prims"; "l_Forall"]
+let squash_qn    = ["Prims"; "squash"]
+
+let int_lid      = ["Prims"; "int"]
+let bool_lid     = ["Prims"; "bool"]
+let unit_lid     = ["Prims"; "unit"]
+
+let add_qn       = ["Prims"; "op_Addition"]
+let neg_qn       = ["Prims"; "op_Minus"]
+let minus_qn     = ["Prims"; "op_Subtraction"]
+let mult_qn      = ["Prims"; "op_Multiply"]
+let div_qn       = ["Prims"; "op_Division"]
+let lt_qn        = ["Prims"; "op_LessThan"]
+let lte_qn       = ["Prims"; "op_LessThanOrEqual"]
+let gt_qn        = ["Prims"; "op_GreaterThan"]
+let gte_qn       = ["Prims"; "op_GreaterThanOrEqual"]
+let mod_qn       = ["Prims"; "op_Modulus"]
+
+(* Vale related functions*)
+let land_qn    = ["FStar" ; "LArith" ; "logand"]
+let lxor_qn    = ["FStar" ; "LArith" ; "logxor"]
+let shiftl_qn  = ["FStar" ; "LArith" ; "shift_left"]
+let shiftr_qn  = ["FStar" ; "LArith" ; "shift_right"]
+let nat_bv_qn  = ["FStar" ; "BitVector" ; "nat_to_bv"]
+
+
+(* Helpers for dealing with nested applications *)
+let rec collect_app' (args : list term) (t : term) : Tot (term * list term) (decreases t) =
+    match inspect t with
+    | Tv_App l r ->
+        collect_app' (r::args) l
+    | _ -> (t, args)
+
+val collect_app : term -> term * list term
+let collect_app = collect_app' []
+
+let rec mk_app (t : term) (args : list term) : Tot term (decreases args) =
+    match args with
+    | [] -> t
+    | (x::xs) -> mk_app (pack (Tv_App t x)) xs
+
+// TODO: move away
+let rec eqlist (f : 'a -> 'a -> bool) (xs : list 'a) (ys : list 'a) : Tot bool =
+    match xs, ys with
+    | [], [] -> true
+    | x::xs, y::ys -> f x y && eqlist f xs ys
+    | _ -> false
+
+let fv_to_string (fv:fv) : string = String.concat "." (inspect_fv fv)
+
+noeq
+type norm_step =
+    | Simpl
+    | WHNF
+    | Primops
+    | Delta
+
+let compare_fv (f1 f2 : fv) : order =
+    compare_list (fun s1 s2 -> order_from_int (String.compare s1 s2)) (inspect_fv f1) (inspect_fv f2)
+
+let rec compare_const (c1 c2 : const) : order =
+    match c1, c2 with
+    | C_Unit, C_Unit -> Eq
+    | C_Int i, C_Int j -> order_from_int (i - j)
+    | C_True, C_True -> Eq
+    | C_False, C_False -> Eq
+    | C_Unit,  _ -> Lt   | _, C_Unit  -> Gt
+    | C_Int _, _ -> Lt   | _, C_Int _ -> Gt
+    | C_True,  _ -> Lt   | _, C_True  -> Gt
+    | C_False, _ -> Lt   | _, C_False -> Gt
+
+let rec compare_term (s t : term) : order =
+    match inspect s, inspect t with
+    | Tv_Var sv, Tv_Var tv ->
+        compare_binder sv tv
+
+    | Tv_FVar sv, Tv_FVar tv ->
+        compare_fv sv tv
+
+    | Tv_App h1 a1, Tv_App h2 a2 ->
+        lex (compare_term h1 h2) (fun () -> compare_term a1 a2)
+
+    | Tv_Abs b1 e1, Tv_Abs b2 e2
+    | Tv_Arrow b1 e1, Tv_Arrow b2 e2
+    | Tv_Refine b1 e1, Tv_Refine b2 e2 ->
+        lex (compare_binder b1 b2) (fun () -> compare_term e1 e2)
+
+    | Tv_Type (), Tv_Type () ->
+        Eq
+
+    | Tv_Const c1, Tv_Const c2 ->
+        compare_const c1 c2
+
+    | Tv_Unknown, Tv_Unknown ->
+        Eq
+
+    // From here onwards, they must have different constructors. Order them arbitrarilly as in the definition.
+    | Tv_Var _, _      -> Lt   | _, Tv_Var _      -> Gt
+    | Tv_FVar _, _     -> Lt   | _, Tv_FVar _     -> Gt
+    | Tv_App _ _, _    -> Lt   | _, Tv_App _ _    -> Gt
+    | Tv_Abs _ _, _    -> Lt   | _, Tv_Abs _ _    -> Gt
+    | Tv_Arrow _ _, _  -> Lt   | _, Tv_Arrow _ _  -> Gt
+    | Tv_Type (), _    -> Lt   | _, Tv_Type ()    -> Gt
+    | Tv_Refine _ _, _ -> Lt   | _, Tv_Refine _ _ -> Gt
+    | Tv_Const _, _    -> Lt   | _, Tv_Const _    -> Gt
+    | Tv_Unknown, _    -> Lt   | _, Tv_Unknown    -> Gt
